# Oppgaver

:::::{grid} 1 1 2 2
---
gutter: 3
---


::::{grid-item-card}
---
link: ./kvadratsetningene/oppgaver
link-type: doc
---
**Oppgaver: Kvadratsetningene**

^^^

$$
(x + 2)^2 = x^2 + 4x + 4
$$

$$
(x - 1)^2 = x^2 - 2x + 1
$$

$$
(x - 2)(x + 2) = x^2 - 4
$$

::::

::::{grid-item-card}
---
link: ./fullstendig_kvadraters_metode/oppgaver
link-type: doc
---
**Oppgaver: Fullstendig kvadraters metode**

^^^

$$
x^2 + 2x + 4 = (x + 1)^2 + 3
$$

$$
x^2 - 4x - 9 = (x - 2)^2 - 13
$$

$$
x^2 + 6x + 9 = (x + 3)^2 + 0
$$

::::


::::{grid-item-card}
---
link: ./blandet/oppgaver
link-type: doc
---
**Blandede oppgaver**

^^^

:::{figure} ./fullstendig_kvadraters_metode/figurer/teori/fullstendig_kvadrat.svg
---
width: 100%
---
:::

::::

:::::